Reorganize Program and Classes theories. Requiring Setoid no longer sets implicits for left, inl or eq, hence some theories had to be changed again. It should make some user contribs compile again too. Also do not import functional extensionality when importing Program.Basics, add a Combinators file for proofs requiring it and a Syntax file for the implicit settings. Move Classes.Relations to Classes.RelationClasses to avoid name clash warnings as advised by Hugo and Pierre.
git-svn-id: svn+ssh://scm.gforge.inria.fr/svn/coq/trunk@10681 85f007b7-540e-0410-9357-904b9bb8a0f7

theories/Classes/RelationClasses.v
@@ -17,14 +17,12 @@
 (* $Id: FSetAVL_prog.v 616 2007-08-08 12:28:10Z msozeau $ *)
 
 Require Export Coq.Classes.Init.
-Require Import Coq.Program.Program.
+Require Import Coq.Program.Basics.
+Require Import Coq.Program.Tactics.
+Require Export Coq.Relations.Relation_Definitions.
 
 Set Implicit Arguments.
 Unset Strict Implicit.
-
-(* Notation "'relation' A " := (A -> A -> Prop) (at level 0). *)
-
-Definition relation A := A -> A -> Prop.
 
 (** Default relation on a given support. *)
 
@@ -35,14 +33,12 @@ Class DefaultRelation A (R : relation A).
 Definition default_relation [ DefaultRelation A R ] : relation A := R.
 
 (** A notation for applying the default relation to [x] and [y]. *)
+
 Notation " x ===def y " := (default_relation x y) (at level 70, no associativity).
 
-Definition inverse A (R : relation A) : relation A := fun x y => R y x.
+Definition inverse {A} : relation A -> relation A := flip.
 
-Lemma inverse_inverse : forall A (R : relation A), inverse (inverse R) = R.
-Proof. intros ; unfold inverse. apply (flip_flip R). Qed.
-
-Definition complement A (R : relation A) : relation A := fun x y => R x y -> False.
+Definition complement {A} (R : relation A) : relation A := fun x y => R x y -> False.
 
 (** These are convertible. *)
 
@@ -355,7 +351,7 @@ Program Instance [ eq : Equivalence A eqA, Antisymmetric eq (R : relation A) ] =
 
 (** Leibinz equality [eq] is an equivalence relation. *)
 
-Program Instance eq_equivalence : Equivalence A eq.
+Program Instance eq_equivalence : Equivalence A (@eq A).
 
 (** Logical equivalence [iff] is an equivalence relation. *)
 
