theories/Program/Basics.v
@@ -1,4 +1,3 @@
-(* -*- coq-prog-args: ("-emacs-U" "-nois") -*- *)
 (************************************************************************)
 (*  v      *   The Coq Proof Assistant  /  The Coq Development Team     *)
 (* <O___,, * CNRS-Ecole Polytechnique-INRIA Futurs-Universite Paris Sud *)
@@ -7,133 +6,50 @@
 (*         *       GNU Lesser General Public License Version 2.1        *)
 (************************************************************************)
 
-(* Standard functions and proofs about them.
+(* Standard functions and combinators.
+ * Proofs about them require functional extensionality and can be found in [Combinators].
+ *
  * Author: Matthieu Sozeau
  * Institution: LRI, CNRS UMR 8623 - UniversitÃcopyright Paris Sud
  *              91405 Orsay, France *)
 
 (* $Id: FSetAVL_prog.v 616 2007-08-08 12:28:10Z msozeau $ *)
 
-Set Implicit Arguments.
-Unset Strict Implicit.
+(** The polymorphic identity function. *)
 
-Require Export Coq.Program.FunctionalExtensionality.
+Definition id {A} := fun x : A => x.
 
-Notation  " 'λ' x : T , y " := (fun x:T => y) (at level 100, x,T,y at level 10, no associativity) : program_scope.
+(** Function composition. *)
 
-Open Local Scope program_scope.
-
-Definition id {A} := λ x : A, x.
-
-Definition compose {A B C} (g : B -> C) (f : A -> B) := λ x : A , g (f x).
+Definition compose {A B C} (f : A -> B) (g : B -> C) := fun x : A => g (f x).
 
 Hint Unfold compose.
 
-Notation " g ∘ f " := (compose g f)  (at level 50, left associativity) : program_scope.
+Notation " g ∘ f " := (compose f g)  (at level 50, left associativity) : program_scope.
 
-Lemma compose_id_left : forall A B (f : A -> B), id ∘ f = f.
-Proof.
-  intros.
-  unfold id, compose.
-  symmetry ; apply eta_expansion.
-Qed.
+Open Local Scope program_scope.
 
-Lemma compose_id_right : forall A B (f : A -> B), f ∘ id = f.
-Proof.
-  intros.
-  unfold id, compose.
-  symmetry ; apply eta_expansion.
-Qed.
-
-Lemma compose_assoc : forall A B C D (f : A -> B) (g : B -> C) (h : C -> D), 
-  h ∘ g ∘ f = h ∘ (g ∘ f).
-Proof.
-  intros.
-  reflexivity.
-Qed.
-
-Hint Rewrite @compose_id_left @compose_id_right @compose_assoc : core.
+(** [arrow A B] represents the non-dependent function space between [A] and [B]. *)
 
 Definition arrow (A B : Type) := A -> B.
 
+(** [impl A B] represents the logical implication of [B] by [A]. *)
+
 Definition impl (A B : Prop) : Prop := A -> B.
 
-(* Notation " f  x " := (f x) (at level 100, x at level 200, only parsing) : program_scope. *)
+(** The constant function [const a] always returns [a]. *)
 
-Definition const {A B} (a : A) := fun x : B => a.
+Definition const {A B} (a : A) := fun _ : B => a.
+
+(** The [flip] combinator reverses the first two arguments of a function. *)
 
 Definition flip {A B C} (f : A -> B -> C) x y := f y x.
 
-Lemma flip_flip : forall A B C (f : A -> B -> C), flip (flip f) = f.
-Proof.
-  unfold flip.
-  intros.
-  extensionality x ; extensionality y.
-  reflexivity.
-Qed.
+(** [apply f x] simply applies [f] to [x]. *)
 
 Definition apply {A B} (f : A -> B) (x : A) := f x.
 
-(** Notations for the unit type and value. *)
+(** Curryfication of [prod] is defined in [Logic.Datatypes]. *)
 
-Notation " () " := Datatypes.unit : type_scope.
-Notation " () " := tt.
-
-(** Set maximally inserted implicit arguments for standard definitions. *)
-
-Implicit Arguments eq [[A]].
-
-Implicit Arguments Some [[A]].
-Implicit Arguments None [[A]].
-
-Implicit Arguments inl [[A] [B]].
-Implicit Arguments inr [[A] [B]].
-
-Implicit Arguments left [[A] [B]].
-Implicit Arguments right [[A] [B]].
-
-(** Curryfication. *)
-
-Definition curry {a b c} (f : a -> b -> c) (p : prod a b) : c :=
-  let (x, y) := p in f x y.
-
-Definition uncurry {a b c} (f : prod a b -> c) (x : a) (y : b) : c :=
-  f (x, y).
-
-Lemma uncurry_curry : forall a b c (f : a -> b -> c), uncurry (curry f) = f.
-Proof.
-  simpl ; intros.
-  unfold uncurry, curry.
-  extensionality x ; extensionality y.
-  reflexivity.
-Qed.
-
-Lemma curry_uncurry : forall a b c (f : prod a b -> c), curry (uncurry f) = f.
-Proof.
-  simpl ; intros.
-  unfold uncurry, curry.
-  extensionality x. 
-  destruct x ; simpl ; reflexivity.
-Qed.
-
-(** n-ary exists ! *)
-
-Notation " 'exists' x y , p" := (ex (fun x => (ex (fun y => p))))
-  (at level 200, x ident, y ident, right associativity) : type_scope.
-
-Notation " 'exists' x y z , p" := (ex (fun x => (ex (fun y => (ex (fun z => p))))))
-  (at level 200, x ident, y ident, z ident, right associativity) : type_scope.
-
-Notation " 'exists' x y z w , p" := (ex (fun x => (ex (fun y => (ex (fun z => (ex (fun w => p))))))))
-  (at level 200, x ident, y ident, z ident, w ident, right associativity) : type_scope.
-
-Tactic Notation "exist" constr(x) := exists x.
-Tactic Notation "exist" constr(x) constr(y) := exists x ; exists y.
-Tactic Notation "exist" constr(x) constr(y) constr(z) := exists x ; exists y ; exists z.
-Tactic Notation "exist" constr(x) constr(y) constr(z) constr(w) := exists x ; exists y ; exists z ; exists w.
-
-(* Notation " 'Σ' x : T , p" := (sigT (fun x : T => p)) *)
-(*   (at level 200, x ident, y ident, right associativity) : program_scope. *)
-
-(* Notation " 'Π' x : T , p " := (forall x : T, p) *)
-(*   (at level 200, x ident, right associativity) : program_scope. *)
+Implicit Arguments prod_curry [[A] [B] [C]].
+Implicit Arguments prod_uncurry [[A] [B] [C]].
