theories/Classes/Equivalence.v
@@ -8,7 +8,6 @@
 (************************************************************************)
 
 (* Typeclass-based setoids, tactics and standard instances.
-   TODO: explain clrewrite, clsubstitute and so on.
  
    Author: Matthieu Sozeau
    Institution: LRI, CNRS UMR 8623 - Universit√copyright Paris Sud
@@ -17,10 +16,10 @@
 (* $Id: FSetAVL_prog.v 616 2007-08-08 12:28:10Z msozeau $ *)
 
 Require Export Coq.Program.Basics.
-Require Import Coq.Program.Program.
+Require Import Coq.Program.Tactics.
 
 Require Import Coq.Classes.Init.
-Require Export Coq.Classes.Relations.
+Require Export Coq.Classes.RelationClasses.
 Require Export Coq.Classes.Morphisms.
 Require Export Coq.Classes.SetoidTactics.
 
