theories/Program/Combinators.v
@@ -1,0 +1,71 @@
+(************************************************************************)
+(*  v      *   The Coq Proof Assistant  /  The Coq Development Team     *)
+(* <O___,, * CNRS-Ecole Polytechnique-INRIA Futurs-Universite Paris Sud *)
+(*   \VV/  **************************************************************)
+(*    //   *      This file is distributed under the terms of the       *)
+(*         *       GNU Lesser General Public License Version 2.1        *)
+(************************************************************************)
+
+(* Proofs about standard combinators, exports functional extensionality.
+ *
+ * Author: Matthieu Sozeau
+ * Institution: LRI, CNRS UMR 8623 - UniversitÃcopyright Paris Sud
+ *              91405 Orsay, France *)
+
+Require Import Coq.Program.Basics.
+Require Export Coq.Program.FunctionalExtensionality.
+
+Open Scope program_scope.
+
+(** Composition has [id] for neutral element and is associative. *)
+
+Lemma compose_id_left : forall A B (f : A -> B), id ∘ f = f.
+Proof.
+  intros.
+  unfold id, compose.
+  symmetry. apply eta_expansion.
+Qed.
+
+Lemma compose_id_right : forall A B (f : A -> B), f ∘ id = f.
+Proof.
+  intros.
+  unfold id, compose.
+  symmetry ; apply eta_expansion.
+Qed.
+
+Lemma compose_assoc : forall A B C D (f : A -> B) (g : B -> C) (h : C -> D), 
+  h ∘ g ∘ f = h ∘ (g ∘ f).
+Proof.
+  intros.
+  reflexivity.
+Qed.
+
+Hint Rewrite @compose_id_left @compose_id_right @compose_assoc : core.
+
+(** [flip] is involutive. *)
+
+Lemma flip_flip : forall A B C, @flip A B C ∘ flip = id.
+Proof.
+  unfold flip, compose.
+  intros.
+  extensionality x ; extensionality y ; extensionality z.
+  reflexivity.
+Qed.
+
+(** [prod_curry] and [prod_uncurry] are each others inverses. *)
+
+Lemma prod_uncurry_curry : forall A B C, @prod_uncurry A B C ∘ prod_curry = id.
+Proof.
+  simpl ; intros.
+  unfold prod_uncurry, prod_curry, compose.
+  extensionality x ; extensionality y ; extensionality z.
+  reflexivity.
+Qed.
+
+Lemma prod_curry_uncurry : forall A B C, @prod_curry A B C ∘ prod_uncurry = id.
+Proof.
+  simpl ; intros.
+  unfold prod_uncurry, prod_curry, compose.
+  extensionality x ; extensionality p.
+  destruct p ; simpl ; reflexivity.
+Qed.
