theories/Program/Program.v
@@ -3,3 +3,5 @@ Require Export Coq.Program.Wf.
 Require Export Coq.Program.Equality.
 Require Export Coq.Program.Subset.
 Require Export Coq.Program.Basics.
+Require Export Coq.Program.Combinators.
+Require Export Coq.Program.Syntax.
