theories/Program/Syntax.v
@@ -1,0 +1,58 @@
+(* -*- coq-prog-args: ("-emacs-U" "-nois") -*- *)
+(************************************************************************)
+(*  v      *   The Coq Proof Assistant  /  The Coq Development Team     *)
+(* <O___,, * CNRS-Ecole Polytechnique-INRIA Futurs-Universite Paris Sud *)
+(*   \VV/  **************************************************************)
+(*    //   *      This file is distributed under the terms of the       *)
+(*         *       GNU Lesser General Public License Version 2.1        *)
+(************************************************************************)
+
+(* Custom notations and implicits for Coq prelude definitions.
+ *
+ * Author: Matthieu Sozeau
+ * Institution: LRI, CNRS UMR 8623 - UniversitÃcopyright Paris Sud
+ *              91405 Orsay, France *)
+
+(** Unicode lambda abstraction, does not work with factorization of lambdas. *)
+
+Notation  " 'λ' x : T , y " := (fun x:T => y) (at level 100, x,T,y at level 10, no associativity) : program_scope.
+
+(** Notations for the unit type and value. *)
+
+Notation " () " := Datatypes.unit : type_scope.
+Notation " () " := tt.
+
+(** Set maximally inserted implicit arguments for standard definitions. *)
+
+Implicit Arguments eq [[A]].
+
+Implicit Arguments Some [[A]].
+Implicit Arguments None [[A]].
+
+Implicit Arguments inl [[A] [B]].
+Implicit Arguments inr [[A] [B]].
+
+Implicit Arguments left [[A] [B]].
+Implicit Arguments right [[A] [B]].
+
+(** n-ary exists ! *)
+
+Notation " 'exists' x y , p" := (ex (fun x => (ex (fun y => p))))
+  (at level 200, x ident, y ident, right associativity) : type_scope.
+
+Notation " 'exists' x y z , p" := (ex (fun x => (ex (fun y => (ex (fun z => p))))))
+  (at level 200, x ident, y ident, z ident, right associativity) : type_scope.
+
+Notation " 'exists' x y z w , p" := (ex (fun x => (ex (fun y => (ex (fun z => (ex (fun w => p))))))))
+  (at level 200, x ident, y ident, z ident, w ident, right associativity) : type_scope.
+
+Tactic Notation "exist" constr(x) := exists x.
+Tactic Notation "exist" constr(x) constr(y) := exists x ; exists y.
+Tactic Notation "exist" constr(x) constr(y) constr(z) := exists x ; exists y ; exists z.
+Tactic Notation "exist" constr(x) constr(y) constr(z) constr(w) := exists x ; exists y ; exists z ; exists w.
+
+(* Notation " 'Σ' x : T , p" := (sigT (fun x : T => p)) *)
+(*   (at level 200, x ident, y ident, right associativity) : program_scope. *)
+
+(* Notation " 'Π' x : T , p " := (forall x : T, p) *)
+(*   (at level 200, x ident, right associativity) : program_scope. *)
